Almost done with finishing off necessary proofs and automation updates for new model check search procedure.

src/ModelCheck/InvariantSearch.v
@@ -19,12 +19,13 @@ From SPICY Require Import
 
      Theory.KeysTheory
 
-     ModelCheck.UniverseEqAutomation
-     ModelCheck.SafeProtocol
+     ModelCheck.InvariantSearchLemmas
      ModelCheck.ProtocolFunctions
      ModelCheck.RealWorldStepLemmas
+     ModelCheck.SafeProtocol
      ModelCheck.SilentStepElimination
      ModelCheck.SteppingTactics
+     ModelCheck.UniverseEqAutomation
 .
 
 From SPICY Require IdealWorld RealWorld.
@@ -88,73 +89,9 @@ Ltac eq1 :=
     | [ H : realServer _ _ _ = _ |- _ ] => erewrite unroll_realserver_step in H by reflexivity
     end.
 
-Lemma lookup_in_merge_perm :
-  forall kid (m m' : key_perms),
-    m $k++ m' $? kid = match m $? kid with
-                       | Some p => match m' $? kid with
-                                  | Some p' => Some (greatest_permission p p')
-                                  | None => Some p
-                                  end
-                       | None => m' $? kid
-                       end.
-Proof.
-  intros; cases (m $? kid); cases (m' $? kid); solve_perm_merges.
-Qed.
-
 Ltac ch := (repeat equality1); subst; rw_step1.
 (* Ltac ch := (repeat equality1); subst; rw_step1. *)
 Ltac chu := repeat ch.
-
-Section RW.
-  Import RealWorld.
-
-
-  Fixpoint compute_na {t} (cmd: user_cmd t) : sigT user_cmd :=
-    match cmd with
-    | Bind c _ => compute_na c
-    | c => existT _ _ c
-    end.
-
-  Lemma compute_na_correct :
-    forall t (cmd : user_cmd t) t__n (cmd__n : user_cmd t__n),
-      compute_na cmd = existT _ _ cmd__n
-      -> nextAction cmd cmd__n.
-  Proof.
-    induct cmd
-    ; try solve [ unfold compute_na; simpl; intros; invert H; econstructor; eauto ].
-
-    intros.
-    constructor.
-    simpl in H0; eauto.
-  Qed.
-
-  Lemma invert_na :
-    forall t (cmd : user_cmd t) t__n (cmd__n : user_cmd t__n),
-      nextAction cmd cmd__n
-      -> compute_na cmd = existT _ _ cmd__n.
-  Proof.
-    induct cmd
-    ; try solve [ intros; unfold compute_na; invert H; split; reflexivity ].
-
-    intros; induct H; eauto.
-    intros; invert H0; eauto.
-  Qed.
-
-  Lemma invert_na' :
-    forall t (cmd : user_cmd t) t__n (cmd__n : user_cmd t__n),
-      nextAction cmd cmd__n
-      -> compute_na cmd = existT _ _ cmd__n
-        /\ projT1 (compute_na cmd) = t__n.
-  Proof.
-
-    induct cmd
-    ; try solve [ intros; unfold compute_na; invert H; split; eauto ].
-
-    intros; induct H; eauto.
-    intros; invert H0; eauto.
-  Qed.
-
-End RW.
 
 Ltac process_map_in_H H :=
   repeat ( (rewrite add_eq_o in H by trivial)           
@@ -465,112 +402,6 @@ Ltac cleanup1 :=
   | [ H : context [[] ++ _] |- _ ] => rewrite !app_nil_l in H
   | [ H : context [_ ++ []] |- _ ] => rewrite !app_nil_r in H
   end || discriminate || eq1.
-
-Inductive NoSilent {A B} (uid : user_id) (U : RealWorld.universe A B) : Prop :=
-| Stuck :
-    (forall U', ~ indexedRealStep uid Silent U U')
-    -> NoSilent uid U.
-
-Lemma NoSilent_no_indexed_silent_step :
-  forall A B uid (U : RealWorld.universe A B), 
-    NoSilent uid U
-    -> forall U',
-      ~ indexedRealStep uid Silent U U'.
-Proof.
-  invert 1; intros; eauto.
-Qed.
-
-Definition propNoSilent {A B} (U U' : RealWorld.universe A B) :=
-  forall uid, NoSilent uid U -> NoSilent uid U'.
-
-Lemma propNoSilent_silent_step :
-  forall A B (U U': RealWorld.universe A B) uid,
-    indexedRealStep uid Silent U U'
-    -> propNoSilent U U'.
-Proof.
-Admitted.
-
-Lemma ssteps_inv_silent' :
-  forall A B st st',
-    (@stepSS A B) ^* st st'
-    -> forall (U U' : RealWorld.universe A B) uid U__i b,
-      st = (U,U__i,b)
-      -> indexedRealStep uid Silent U U'
-      -> (forall uid' U', uid' > uid -> ~ indexedRealStep uid' Silent U U')
-      -> exists U__r,
-          indexedRealStep uid Silent U U__r
-          /\ (  st' = (U,U__i,b)
-               \/  (stepSS (t__adv := B) ^* (U__r,U__i,b) st')
-            )
-          /\ propNoSilent U U__r.
-Proof.
-  intros.
-  subst; invert H.
-  - eexists; eauto 8 using propNoSilent_silent_step.
-  - invert H0; repeat equality1.
-
-    invert H.
-    + apply indexedModelStep_user_step in H6; split_ex; split_ors; subst.
-      * destruct ( uid ==n u_id ); subst.
-        clear H1 H4.
-        
-        eexists; repeat simple apply conj; eauto using propNoSilent_silent_step.
-        exfalso.
-
-        destruct (le_gt_dec u_id uid).
-        assert (uid > u_id) by lia.
-        eapply H5; eauto.
-        eapply H2; eauto.
-        
-      * invert H; invert H4.
-        exfalso.
-        clean_map_lookups
-        ; pose proof (user_step_label_deterministic _ _ _ _ _ _ _ _ _ H7 H8); discriminate.
-
-    + eapply H4 in H1; contradiction.
-Qed.
-
-Lemma ssteps_inv_labeled :
-  forall A B st st' ru,
-    (forall uid U', ~ @indexedRealStep A B uid Silent ru U')
-    -> (@stepSS A B) ^* st st'
-    -> labels_align st
-    -> forall iu b,
-        st = (ru,iu,b)
-        (* -> st' = (ru',iu',b') *)
-        -> st = st'
-          \/ exists uid ru' iu0 iu' ra ia,
-            indexedRealStep uid (Action ra) ru ru'
-            /\ (indexedIdealStep uid Silent) ^* iu iu0
-            /\ indexedIdealStep uid (Action ia) iu0 iu'
-            /\ action_matches (RealWorld.all_ciphers ru) (RealWorld.all_keys ru) (uid,ra) ia
-            /\ (@stepSS A B) ^* (ru',iu',b) st'.
-Proof.
-  intros; subst.
-  invert H0; clear_mislabeled_steps; eauto.
-  right.
-
-  invert H2; repeat equality1.
-  invert H0.
-  - exfalso; eapply H; eauto.
-  - invert H6; try contradiction.
-    clear_mislabeled_steps.
-    eauto 12.
-Qed.
-
-
-Lemma all_users_NoSilent_no_indexed_silent_step :
-  forall A B uid (U : RealWorld.universe A B),
-    (forall uid ud, U.(RealWorld.users) $? uid = Some ud -> NoSilent uid U)
-    -> forall U',
-      ~ indexedRealStep uid Silent U U'.
-Proof.
-  intros.
-  unfold not; intros.
-  generalize H0; invert H0.
-  apply H in H1.
-  eapply NoSilent_no_indexed_silent_step; eauto.
-Qed.
 
 Ltac print_nosilents :=
   repeat
