src/ModelCheck/InvariantSearchLemmas.v
@@ -1,0 +1,435 @@
+(*
+ * © 2021 Massachusetts Institute of Technology.
+ * MIT Proprietary, Subject to FAR52.227-11 Patent Rights - Ownership by the Contractor (May 2014)
+ * SPDX-License-Identifier: MIT
+ * 
+ *)
+From Coq Require Import
+     List
+     Lia.
+
+From SPICY Require Import
+     MyPrelude
+     Maps
+     Messages
+     Keys
+     Tactics
+     RealWorld
+     SafeProtocol
+     SafetyAutomation
+     Simulation
+
+     ModelCheck.LabelsAlign
+     ModelCheck.ProtocolFunctions
+     ModelCheck.RealWorldStepLemmas
+     ModelCheck.SilentStepElimination
+     ModelCheck.SteppingTactics
+
+     Theory.InvariantsTheory
+     Theory.KeysTheory
+.
+
+Import SafetyAutomation Gen.
+
+Set Implicit Arguments.
+
+Lemma lookup_in_merge_perm :
+  forall kid (m m' : key_perms),
+    m $k++ m' $? kid = match m $? kid with
+                       | Some p => match m' $? kid with
+                                  | Some p' => Some (greatest_permission p p')
+                                  | None => Some p
+                                  end
+                       | None => m' $? kid
+                       end.
+Proof.
+  intros; cases (m $? kid); cases (m' $? kid); solve_perm_merges.
+Qed.
+
+Section RW.
+  Import RealWorld.
+
+  Fixpoint compute_na {t} (cmd: user_cmd t) : sigT user_cmd :=
+    match cmd with
+    | Bind c _ => compute_na c
+    | c => existT _ _ c
+    end.
+
+  Lemma compute_na_correct :
+    forall t (cmd : user_cmd t) t__n (cmd__n : user_cmd t__n),
+      compute_na cmd = existT _ _ cmd__n
+      -> nextAction cmd cmd__n.
+  Proof.
+    induct cmd
+    ; try solve [ unfold compute_na; simpl; intros; invert H; econstructor; eauto ].
+
+    intros.
+    constructor.
+    simpl in H0; eauto.
+  Qed.
+
+  Lemma invert_na :
+    forall t (cmd : user_cmd t) t__n (cmd__n : user_cmd t__n),
+      nextAction cmd cmd__n
+      -> compute_na cmd = existT _ _ cmd__n.
+  Proof.
+    induct cmd
+    ; try solve [ intros; unfold compute_na; invert H; split; reflexivity ].
+
+    intros; induct H; eauto.
+    intros; invert H0; eauto.
+  Qed.
+
+  Lemma invert_na' :
+    forall t (cmd : user_cmd t) t__n (cmd__n : user_cmd t__n),
+      nextAction cmd cmd__n
+      -> compute_na cmd = existT _ _ cmd__n
+        /\ projT1 (compute_na cmd) = t__n.
+  Proof.
+
+    induct cmd
+    ; try solve [ intros; unfold compute_na; invert H; split; eauto ].
+
+    intros; induct H; eauto.
+    intros; invert H0; eauto.
+  Qed.
+
+End RW.
+
+Inductive NoSilent {A B} (uid : user_id) (U : RealWorld.universe A B) : Prop :=
+| Stuck :
+    (forall U', ~ indexedRealStep uid Silent U U')
+    -> NoSilent uid U.
+
+Lemma step_didnt_appear :
+  forall {A B C} suid lbl bd bd',
+
+    step_user lbl suid bd bd'
+    -> forall cs cs' (usrs usrs': honest_users A) (adv adv' : user_data B) gks gks'
+        (cmd cmd' : user_cmd C) uid1 ks ks' qmsgs qmsgs' mycs mycs' ms
+        froms froms' sents sents' cur_n cur_n' cmdc,
+
+      bd = (usrs, adv, cs, gks, ks, qmsgs ++ ms, mycs, froms, sents, cur_n, cmd)
+      -> bd' = (usrs', adv', cs', gks', ks', qmsgs', mycs', froms', sents', cur_n', cmd')
+      -> suid = Some uid1
+      -> lbl = Silent
+      -> usrs $? uid1 = Some {| key_heap := ks;
+                               protocol := cmdc;
+                               msg_heap := qmsgs ++ ms;
+                               c_heap   := mycs;
+                               from_nons := froms;
+                               sent_nons := sents;
+                               cur_nonce := cur_n |}
+      -> forall usrs'' (adv'' : user_data B) cs'' gks'',
+          usrs'' $? uid1 = Some {| key_heap := ks;
+                                   protocol := cmdc;
+                                   msg_heap := qmsgs;
+                                   c_heap   := mycs;
+                                   from_nons := froms;
+                                   sent_nons := sents;
+                                   cur_nonce := cur_n |}
+          -> (forall uid u, usrs'' $? uid = Some u -> exists u', usrs $? uid = Some u')
+          -> (forall cid c, cs'' $? cid = Some c -> cs $? cid = Some c)
+          -> (forall cid c, cs $? cid = Some c -> cs'' $? cid = Some c \/ cs'' $? cid = None)
+          -> (forall kid k, gks $? kid = Some k -> gks'' $? kid = Some k \/ gks'' $? kid = None)
+          -> (forall kid k, gks'' $? kid = Some k -> gks $? kid = Some k)
+          -> keys_and_permissions_good gks'' usrs'' adv''.(key_heap)
+          -> user_cipher_queues_ok cs'' (findUserKeys usrs'') usrs''
+          -> exists bd'',
+              step_user Silent suid
+                        (usrs'', adv'', cs'', gks'', ks, qmsgs, mycs, froms, sents, cur_n, cmd)
+                        bd''.
+Proof.
+  induction 1; inversion 1; inversion 1
+  ; intros
+  ; subst
+  ; try discriminate
+  ; try solve [ eexists; econstructor; eauto ]
+  ; eauto.
+
+  - eapply IHstep_user in H27; eauto.
+    split_ex; eauto.
+    dt x.
+    eexists; econstructor; eauto.
+  - keys_and_permissions_prop.
+    generalize (H12 _ _ H1); generalize (H12 _ _ H2); intros; split_ex.
+    destruct x0; destruct x; clean_map_lookups.
+    apply H41 in H; apply H41 in H0; split_ors; clean_map_lookups.
+    eexists; eapply StepEncrypt with (c_id0 := next_key cs''); eauto using Maps.next_key_not_in.
+  - user_cipher_queues_prop.
+    keys_and_permissions_prop.
+    generalize (H13 _ _ H2); generalize (H13 _ _ H3); intros; split_ex.
+    apply H38 in H; split_ors; clean_map_lookups.
+    eapply H39 in H0; eapply H39 in H1; split_ors; clean_map_lookups.
+    eexists; econstructor; eauto.
+  - keys_and_permissions_prop.
+    apply H39 in H.
+    specialize (H10 _ _ H0); split_ors; clean_map_lookups.
+    eexists; eapply StepSign with (c_id0 := next_key cs''); eauto using Maps.next_key_not_in.
+  - user_cipher_queues_prop.
+    keys_and_permissions_prop.
+    generalize (H11 _ _ H0); intros; split_ex.
+    apply H34 in H; split_ors; clean_map_lookups.
+    eapply H33 in H1; split_ors; clean_map_lookups.
+    eexists; econstructor; eauto.
+  - eexists; eapply StepGenerateKey with (k_id0 := next_key gks''); eauto using Maps.next_key_not_in.
+
+    Unshelve.
+    auto.
+Qed.
+
+Lemma silent_step_then_silent_step_inv :
+  forall {A B} suid lbl bd bd',
+
+    step_user lbl suid bd bd'
+    -> forall cs cs' (usrs usrs': honest_users A) (adv adv' : user_data B) gks gks'
+        (cmd cmd' : user_cmd (Base A)) uid1 ks ks' qmsgs qmsgs' mycs mycs'
+        froms froms' sents sents' cur_n cur_n' cmdc,
+
+      bd = (usrs, adv, cs, gks, ks, qmsgs, mycs, froms, sents, cur_n, cmd)
+      -> bd' = (usrs', adv', cs', gks', ks', qmsgs', mycs', froms', sents', cur_n', cmd')
+      -> suid = Some uid1
+      -> lbl = Silent
+      -> usrs $? uid1 = Some {| key_heap := ks;
+                               protocol := cmdc;
+                               msg_heap := qmsgs;
+                               c_heap   := mycs;
+                               from_nons := froms;
+                               sent_nons := sents;
+                               cur_nonce := cur_n |}
+
+      -> forall uid2 bd2 bd2' cmd2 ks2 qmsgs2 mycs2 froms2 sents2 cur_n2 usrs'' cmdc' ud2,
+
+          step_user Silent (Some uid2)
+                    (usrs'', adv', cs', gks', ks2, qmsgs2, mycs2, froms2, sents2, cur_n2, cmd2)
+                    bd2'
+          -> uid1 <> uid2
+          -> usrs $? uid2 = Some ud2
+          -> bd2 = build_data_step (mkUniverse usrs adv cs gks) ud2
+          -> usrs' $? uid2 = Some {| key_heap := ks2;
+                                    protocol := cmd2;
+                                    msg_heap := qmsgs2;
+                                    c_heap   := mycs2;
+                                    from_nons := froms2;
+                                    sent_nons := sents2;
+                                    cur_nonce := cur_n2 |}
+          -> usrs'' = usrs' $+ (uid1, {| key_heap := ks';
+                                        protocol := cmdc';
+                                        msg_heap := qmsgs';
+                                        c_heap   := mycs';
+                                        from_nons := froms';
+                                        sent_nons := sents';
+                                        cur_nonce := cur_n' |})
+          -> keys_and_permissions_good gks usrs adv.(key_heap)
+          -> user_cipher_queues_ok cs (findUserKeys usrs) usrs
+          -> exists bd2'',
+              step_user Silent (Some uid2) bd2 bd2''
+.
+Proof.
+  induction 1; inversion 1; inversion 1; intros; subst
+  ; autorewrite with find_user_keys in *
+  ; try discriminate
+  ; try solve [
+          dt bd2'; clean_map_lookups
+          ; eapply step_didnt_appear with (ms := [])
+          ; try rewrite app_nil_r
+          ; simpl; eauto
+          ; intros
+          ; clean_map_lookups
+          ; trivial
+          ; destruct (uid1 ==n uid); subst; clean_map_lookups; eauto].
+
+  - eapply IHstep_user in H28; eauto.
+      
+  - dt bd2'; clean_map_lookups
+    ; eapply step_didnt_appear with (ms := [])
+    ; try rewrite app_nil_r
+    ; simpl; eauto.
+
+    clean_map_lookups; trivial.
+    
+    intros; destruct (uid1 ==n uid); subst; clean_map_lookups; eauto.
+    intros; destruct (c_id ==n cid); subst; clean_map_lookups; eauto.
+    intros; destruct (c_id ==n cid); subst; clean_map_lookups; eauto.
+
+  - dt bd2'; clean_map_lookups
+    ; eapply step_didnt_appear with (ms := [])
+    ; try rewrite app_nil_r
+    ; simpl; eauto.
+    
+    clean_map_lookups; trivial.
+    
+    intros; destruct (uid1 ==n uid); subst; clean_map_lookups; eauto.
+    intros; destruct (c_id ==n cid); subst; clean_map_lookups; eauto.
+    intros; destruct (c_id ==n cid); subst; clean_map_lookups; eauto.
+
+  - dt bd2'; clean_map_lookups
+    ; eapply step_didnt_appear with (ms := [])
+    ; try rewrite app_nil_r
+    ; simpl; eauto.
+    
+    clean_map_lookups; trivial.
+    
+    intros; destruct (uid1 ==n uid); subst; clean_map_lookups; eauto.
+    intros; destruct (k_id ==n kid); subst; clean_map_lookups; eauto.
+    intros; destruct (k_id ==n kid); subst; clean_map_lookups; eauto.
+Qed.
+
+Lemma NoSilent_no_indexed_silent_step :
+  forall A B uid (U : RealWorld.universe A B), 
+    NoSilent uid U
+    -> forall U',
+      ~ indexedRealStep uid Silent U U'.
+Proof.
+  invert 1; intros; eauto.
+Qed.
+
+Definition propNoSilent {A B} (U U' : RealWorld.universe A B) :=
+  forall uid, NoSilent uid U -> NoSilent uid U'.
+
+Lemma all_users_NoSilent_no_indexed_silent_step :
+  forall A B uid (U : RealWorld.universe A B),
+    (forall uid ud, U.(RealWorld.users) $? uid = Some ud -> NoSilent uid U)
+    -> forall U',
+      ~ indexedRealStep uid Silent U U'.
+Proof.
+  intros.
+  unfold not; intros.
+  generalize H0; invert H0.
+  apply H in H1.
+  eapply NoSilent_no_indexed_silent_step; eauto.
+Qed.
+
+Lemma silent_step_nochange_other_user_inv :
+  forall {A B C} suid lbl bd bd',
+    step_user lbl suid bd bd'
+    -> forall cs cs' (usrs usrs': honest_users A) (adv adv' : user_data B) gks gks'
+        (cmd cmd' : user_cmd C) ks ks' qmsgs qmsgs' mycs mycs'
+        froms froms' sents sents' cur_n cur_n',
+      bd = (usrs, adv, cs, gks, ks, qmsgs, mycs, froms, sents, cur_n, cmd)
+      -> bd' = (usrs', adv', cs', gks', ks', qmsgs', mycs', froms', sents', cur_n', cmd')
+      -> lbl = Silent
+      -> forall cmdc u_id1 u_id2 ud2,
+          suid = Some u_id1
+          -> u_id1 <> u_id2
+          -> usrs $? u_id1 = Some {| key_heap := ks;
+                                    protocol := cmdc;
+                                    msg_heap := qmsgs;
+                                    c_heap   := mycs;
+                                    from_nons := froms;
+                                    sent_nons := sents;
+                                    cur_nonce := cur_n |}
+          -> usrs' $? u_id2 = Some ud2
+          -> usrs $? u_id2 = Some ud2.
+Proof.
+  induction 1; inversion 1; inversion 1
+  ; intros; subst
+  ; try discriminate
+  ; try solve [ clean_map_lookups; trivial ]
+  ; eauto.
+Qed.
+
+Lemma propNoSilent_silent_step :
+  forall A B (U U': RealWorld.universe A B) uid,
+    indexedRealStep uid Silent U U'
+    -> keys_and_permissions_good U.(all_keys) U.(users) U.(adversary).(key_heap)
+    -> user_cipher_queues_ok U.(all_ciphers) (findUserKeys U.(users)) U.(users)
+    -> propNoSilent U U'.
+Proof.
+  unfold propNoSilent; intros.
+  invert H2.
+  constructor; unfold not; intros.
+
+  destruct (uid ==n uid0); subst.
+
+  apply H3 in H; auto.
+
+  invert H; invert H2.
+  destruct U, userData, userData0.
+  unfold build_data_step, buildUniverse in *; simpl in *; clean_map_lookups.
+
+  pose proof (silent_step_then_silent_step_inv H5).
+  pose proof (silent_step_nochange_other_user_inv H5).
+
+  specialize (H7 _ _ _ _ _ _ _ _ _ _ _ _ _ _ _ _ _ _ _ _ _ _ eq_refl eq_refl eq_refl).
+  specialize (H7 _ _ _ _ eq_refl n H4 H).
+  
+  specialize (H2 _ _ _ _ _ _ _ _ _ _ _ _ _ _ _ _ _ _ _ _ _ _ _ _ eq_refl eq_refl eq_refl eq_refl H4).
+  specialize (H2 _ _ _ _ _ _ _ _ _ _ _ _ _ H6 n H7 eq_refl H eq_refl).
+
+  specialize (H2 H0 H1).
+
+  split_ex.
+  dt x.
+  eapply H3.
+  econstructor; simpl; eauto.
+Qed.
+
+Lemma ssteps_inv_silent' :
+  forall A B st st',
+    (@stepSS A B) ^* st st'
+    -> forall (U U' : RealWorld.universe A B) uid U__i b,
+      st = (U,U__i,b)
+      -> indexedRealStep uid Silent U U'
+      -> (forall uid' U', uid' > uid -> ~ indexedRealStep uid' Silent U U')
+      -> keys_and_permissions_good U.(all_keys) U.(users) U.(adversary).(key_heap)
+      -> user_cipher_queues_ok U.(all_ciphers) (findUserKeys U.(users)) U.(users)
+      -> exists U__r,
+          indexedRealStep uid Silent U U__r
+          /\ (  st' = (U,U__i,b)
+               \/  (stepSS (t__adv := B) ^* (U__r,U__i,b) st')
+            )
+          /\ propNoSilent U U__r.
+Proof.
+  intros.
+  subst; invert H.
+  - eexists; eauto 8 using propNoSilent_silent_step.
+  - invert H0; repeat equality1.
+    invert H.
+    + apply indexedModelStep_user_step in H8; split_ex; split_ors; subst.
+      * destruct ( uid ==n u_id ); subst.
+        clear H1 H6.
+        
+        eexists; repeat simple apply conj; eauto using propNoSilent_silent_step.
+        exfalso.
+
+        destruct (le_gt_dec u_id uid).
+        assert (uid > u_id) by lia.
+        eapply H7; eauto.
+        eapply H2; eauto.
+        
+      * invert H; invert H6.
+        exfalso.
+        clean_map_lookups
+        ; pose proof (user_step_label_deterministic _ _ _ _ _ _ _ _ _ H9 H10); discriminate.
+
+    + eapply H6 in H1; contradiction.
+Qed.
+
+Lemma ssteps_inv_labeled :
+  forall A B st st' ru,
+    (forall uid U', ~ @indexedRealStep A B uid Silent ru U')
+    -> (@stepSS A B) ^* st st'
+    -> labels_align st
+    -> forall iu b,
+        st = (ru,iu,b)
+        (* -> st' = (ru',iu',b') *)
+        -> st = st'
+          \/ exists uid ru' iu0 iu' ra ia,
+            indexedRealStep uid (Action ra) ru ru'
+            /\ (indexedIdealStep uid Silent) ^* iu iu0
+            /\ indexedIdealStep uid (Action ia) iu0 iu'
+            /\ action_matches (RealWorld.all_ciphers ru) (RealWorld.all_keys ru) (uid,ra) ia
+            /\ (@stepSS A B) ^* (ru',iu',b) st'.
+Proof.
+  intros; subst.
+  invert H0; clear_mislabeled_steps; eauto.
+  right.
+
+  invert H2; repeat equality1.
+  invert H0.
+  - exfalso; eapply H; eauto.
+  - invert H6; try contradiction.
+    clear_mislabeled_steps.
+    eauto 12.
+Qed.
